disk-betree/CrashTypes.dfy
@@ -1,4 +1,4 @@
-abstract module CrashTypes {
+module CrashTypes {
   datatype CrashableUIOp<UIOp> = 
     | CrashOp
     | NormalOp(uiop: UIOp)
